\section*{Ejercicio 32}
Mostrar que 
\begin{equation*}
    {{\omega_0}^1} = - {\omega^0}_1
\end{equation*}
Obteniendo el termino ${{\omega_0}^1}$
\begin{align*}
    {\omega_0}^1 =& g_{0\beta} \omega^{\beta 1}\\
     =& g_{00} \omega^{01}  +g_{01} \omega^{11}  +g_{02} \omega^{21}  +g_{03} \omega^{31}  \\
    =& g_{00} \omega^{01}\\
      =& \omega^{01}  
\end{align*}
obtiendo el termino ${\omega^0}_1$
\begin{align*}
    {\omega^0}_1 =&g_{1\beta}\omega^{0\beta} \\
    =& g_{10} \omega^{00}  +g_{11} \omega^{01}  +g_{21} \omega^{02}  +g_{31} \omega^{03}  \\
    =& g_{11} \omega^{01}\\
    =& -\omega^{01}
\end{align*}
por lo tanto
\begin{equation*}
    {{\omega_0}^1} = - {\omega^0}_1
\end{equation*}