\section*{Ejercio 39}
Mostrar que
\begin{equation*}
    {\bar{\psi}}'({x}') \gamma^\nu {\psi}' ({x}') = {a^\nu}_\mu \bar{\psi} \gamma^\mu \psi
\end{equation*}
Se sabe que:
\begin{equation*}
    {\bar{\psi}}'({x}') = \bar{\psi} \hat{S}^{-1} \qquad {\psi}'({x}')=\hat{S}\psi(x) 
\end{equation*}
entonces
\begin{equation*}
    {\bar{\psi}}'({x}') \gamma^\nu {\psi}' ({x}')  =  \bar{\psi} \hat{S}^{-1}  \gamma^\nu \hat{S}\psi(x) 
\end{equation*}
como 
\begin{equation*}
    \hat{S}^{-1}  \gamma^\nu \hat{S} = {a^\nu}_\mu \gamma^\mu
\end{equation*}
entonces 
\begin{align*}
    {\bar{\psi}}'({x}') \gamma^\nu {\psi}' ({x}') =& \bar{\psi} {a^\nu}_\mu \gamma^\mu\psi(x)  \\
    =& {a^\nu}_\mu \bar{\psi} \gamma^\mu \psi
\end{align*}
por lo tanto
\begin{equation*}
    {\bar{\psi}}'({x}') \gamma^\nu {\psi}' ({x}') = {a^\nu}_\mu \bar{\psi} \gamma^\mu \psi
\end{equation*}