\section*{Ejercicio 33}
Verificar ${x^1}',{x^2}',{x^3}'$\\
Se tiene que
\begin{equation*}
    {x^\nu}'=\left[\delta_\mu^\nu - \Delta \beta {\delta_1}^\nu {\delta^0}_\mu - \Delta \beta{\delta_0}^\nu \delta_\mu^1\right]x^\mu
\end{equation*}
para ${x^1}'$ se tiene que:
\begin{align*}
    {x^1}'=&\left[\delta_\mu^1 - \Delta \beta {\delta_1}^1 {\delta^0}_\mu - \Delta \beta{\delta_0}^1 \delta_\mu^1\right]x^\mu\\
=&\left[\delta_\mu^1 - \Delta\beta \delta_\mu^0\right] x^\mu\\
=&x^1-\Delta\beta x^0
\end{align*}
para ${x^2}'$
\begin{align*}
    {x^2}'=&\left[\delta_\mu^2 - \Delta \beta {\delta_1}^2 {\delta^0}_\mu - \Delta \beta{\delta_0}^2 \delta_\mu^1\right]x^\mu\\
=& \delta_\mu^2x^\mu\\
=& x^2
\end{align*}
para ${x^3}'$
\begin{align*}
    {x^3}'=&\left[\delta_\mu^3 - \Delta \beta {\delta_1}^3 {\delta^0}_\mu - \Delta \beta{\delta_0}^3 \delta_\mu^1\right]x^\mu\\
=& \delta_\mu^3x^\mu\\
=& x^3
\end{align*}