\section*{Ejercicio 17}
Mostras que
\begin{itemize}
    \item $H(+)=E_{pn}$
    \item $H(-)=E_{pn}$
\end{itemize}
Se tiene que:
\begin{equation*}
    \psi_n (\pm) = \sqrt{\frac{m_0c^2}{L^3E_{\rho m}}} exp\left[\frac{i}{\hbar}\left(\vec{p}\cdot \vec{x}\mp E_{\rho n}t\right)\right]
\end{equation*}
y la operaci√≥n H es definida como:
\begin{equation*}
    H=\int\limits_{L^B} T_0^0(n,\pm) dx^3
\end{equation*}
donde 
\begin{equation*}
    T_0^0 = \frac{\hbar^2}{2m_0} \left[\frac{1}{c^2} \frac{\partial \psi^*}{\partial t}\frac{\partial \psi}{\partial t}+ \left(\nabla \psi^*\right)\cdot \left(\nabla \psi \right)+ \frac{m_0^2c^2}{\hbar^2} \psi^* \psi \right]  
\end{equation*}
Para $H(+)$, calculando $ \frac{\partial \psi^*}{\partial t}$  y $ \frac{\partial \psi}{\partial t}$:
\begin{align*}
    \frac{\partial \psi^*}{\partial t} = \frac{i}{\hbar} E_{\rho n} \psi^* &\qquad  \frac{\partial \psi}{\partial t} = \frac{-i}{\hbar} E_{\rho n} \psi\\
    \frac{1}{c^2}  \frac{\partial \psi^*}{\partial t} \frac{\partial \psi}{\partial t} &= \frac{E_{\rho n}^2}{\hbar^2c^2} \psi^* \psi\\
    &= \frac{E_{\rho n}m_0}{\hbar^2 L^3}
\end{align*}
Calculando $\nabla \psi^*$ y $\nabla \psi$
\begin{align*}
    \nabla \psi^* = \frac{-i\vec{P}}{\hbar}\psi^* &\qquad \nabla \psi = \frac{i\vec{P}}{\hbar} \psi\\
    \left(\nabla \psi^*\right) \cdot \left(\nabla \psi\right) &=\frac{\vec{p}\cdot \vec{p}}{\hbar^2} \psi^* \psi \\
    &= \frac{P^2}{\hbar^2} \left(\frac{m_0c^2}{L^3 E_{\rho n}}\right)\\
    &= \frac{1}{c^2 \hbar^2} \left(\frac{m_0c^2}{L^3 E_{\rho n}}\right) (E_{\rho n}^2-m_0^2c^4)\\
    &= \left(\frac{m_0}{L^3 E_{\rho n }\hbar^2}\right) (E_{\rho n}^2-m^2c^4)
\end{align*}
por lo tanto
\begin{align*}
    T_0^0 &= \frac{\hbar^2}{2m_0} \left[\frac{1}{c^2} \frac{\partial \psi^*}{\partial t}\frac{\partial \psi}{\partial t}+ \left(\nabla \psi^*\right)\cdot \left(\nabla \psi \right)+ \frac{m_0^2c^2}{\hbar^2} \psi^* \psi \right]  \\
    &= \frac{\hbar^2}{2m_0} \left[\frac{E_{\rho n}m_0}{\hbar^2 L^3} + \left(\frac{m_0}{L^3 E_{\rho n }\hbar^2}\right) (E_{\rho n}^2-m_0^2c^4)+\left(\frac{m_0}{L^3 E_{\rho n }\hbar^2}\right)(m_0^2c^4)\right]\\
    & = \frac{E_{\rho n}}{L^3}
\end{align*}
entonces
\begin{align*}
    \int\limits_{L^B}   T_0^0(n,+) dx^3 &= \int\limits_{L^B}  \frac{E_{\rho n}}{L^3} dV \\
    &= \frac{E_{\rho n}}{L^3} \int\limits_{L^B} dV \\
    &= E_{\rho n}
\end{align*}
por lo tanto
\begin{equation*}
    H(+)= E_{\rho n}
\end{equation*}


Para $H(-)$, calculando $ \frac{\partial \psi^*}{\partial t}$  y $ \frac{\partial \psi}{\partial t}$:
\begin{align*}
    \frac{\partial \psi^*}{\partial t} = \frac{-i}{\hbar} E_{\rho n} \psi^* &\qquad  \frac{\partial \psi}{\partial t} = \frac{i}{\hbar} E_{\rho n} \psi\\
    \frac{1}{c^2}  \frac{\partial \psi^*}{\partial t} \frac{\partial \psi}{\partial t} &= \frac{E_{\rho n}^2}{\hbar^2c^2} \psi^* \psi\\
    &= \frac{E_{\rho n}m_0}{\hbar^2 L^3}
\end{align*}
Calculando $\nabla \psi^*$ y $\nabla \psi$
\begin{align*}
    \nabla \psi^* = \frac{-i\vec{P}}{\hbar}\psi^* &\qquad \nabla \psi = \frac{i\vec{P}}{\hbar} \psi\\
    \left(\nabla \psi^*\right) \cdot \left(\nabla \psi\right) &=\frac{\vec{p}\cdot \vec{p}}{\hbar^2} \psi^* \psi \\
    &= \frac{P^2}{\hbar^2} \left(\frac{m_0c^2}{L^3 E_{\rho n}}\right)\\
    &= \frac{1}{c^2 \hbar^2} \left(\frac{m_0c^2}{L^3 E_{\rho n}}\right) (E_{\rho n}^2-m_0^2c^4)\\
    &= \left(\frac{m_0}{L^3 E_{\rho n }\hbar^2}\right) (E_{\rho n}^2-m^2c^4)
\end{align*}
por lo tanto
\begin{align*}
    T_0^0 &= \frac{\hbar^2}{2m_0} \left[\frac{1}{c^2} \frac{\partial \psi^*}{\partial t}\frac{\partial \psi}{\partial t}+ \left(\nabla \psi^*\right)\cdot \left(\nabla \psi \right)+ \frac{m_0^2c^2}{\hbar^2} \psi^* \psi \right]  \\
    &= \frac{\hbar^2}{2m_0} \left[\frac{E_{\rho n}m_0}{\hbar^2 L^3} + \left(\frac{m_0}{L^3 E_{\rho n }\hbar^2}\right) (E_{\rho n}^2-m_0^2c^4)+\left(\frac{m_0}{L^3 E_{\rho n }\hbar^2}\right)(m_0^2c^4)\right]\\
    & = \frac{E_{\rho n}}{L^3}
\end{align*}
entonces
\begin{align*}
    \int\limits_{L^B}   T_0^0(n,-) dx^3 &= \int\limits_{L^B}  \frac{E_{\rho n}}{L^3} dV \\
    &= \frac{E_{\rho n}}{L^3} \int\limits_{L^B} dV \\
    &= E_{\rho n}
\end{align*}
por lo tanto
\begin{equation*}
    H(-)= E_{\rho n}
\end{equation*}